NuSys.thy
@@ -112,37 +112,31 @@ in Attrib.add_del cong_add cong_del end\<close>
 
 subsection \<open>Cast\<close>
 
-definition Cast :: " 'a set \<Rightarrow> 'a set \<Rightarrow> bool \<Rightarrow> bool \<Rightarrow> bool " ("(2\<^bold>c\<^bold>a\<^bold>s\<^bold>t _ \<longmapsto> _/ \<^bold>w\<^bold>i\<^bold>t\<^bold>h _ \<^bold>w\<^bold>h\<^bold>e\<^bold>n _)" [13,13,13,13] 12)
-  where "(\<^bold>c\<^bold>a\<^bold>s\<^bold>t A \<longmapsto> B \<^bold>w\<^bold>i\<^bold>t\<^bold>h P \<^bold>w\<^bold>h\<^bold>e\<^bold>n Q) \<longleftrightarrow> (\<forall>v. Q \<longrightarrow> v \<in> A \<longrightarrow> v \<in> B \<and> P)"
-consts SimpleCast1 :: " 'a set \<Rightarrow> 'a set \<Rightarrow> bool \<Rightarrow> bool " ("(2\<^bold>c\<^bold>a\<^bold>s\<^bold>t _/ \<longmapsto> _ \<^bold>w\<^bold>i\<^bold>t\<^bold>h _)" [13,13,13] 12)
-consts SimpleCast2 :: " 'a set \<Rightarrow> 'a set \<Rightarrow> bool \<Rightarrow> bool " ("(2\<^bold>c\<^bold>a\<^bold>s\<^bold>t _/ \<longmapsto> _ \<^bold>w\<^bold>h\<^bold>e\<^bold>n _)" [13,13,13] 12)
-consts SimpleCast3 :: " 'a set \<Rightarrow> 'a set \<Rightarrow> bool " ("(2\<^bold>c\<^bold>a\<^bold>s\<^bold>t _/ \<longmapsto> _)" [13,13] 12)
-translations
-  "(\<^bold>c\<^bold>a\<^bold>s\<^bold>t A \<longmapsto> B)" == "(\<^bold>c\<^bold>a\<^bold>s\<^bold>t A \<longmapsto> B \<^bold>w\<^bold>i\<^bold>t\<^bold>h CONST True \<^bold>w\<^bold>h\<^bold>e\<^bold>n CONST True)"
-  "(\<^bold>c\<^bold>a\<^bold>s\<^bold>t A \<longmapsto> B \<^bold>w\<^bold>i\<^bold>t\<^bold>h P)" == "(\<^bold>c\<^bold>a\<^bold>s\<^bold>t A \<longmapsto> B \<^bold>w\<^bold>i\<^bold>t\<^bold>h P \<^bold>w\<^bold>h\<^bold>e\<^bold>n CONST True)"
-  "(\<^bold>c\<^bold>a\<^bold>s\<^bold>t A \<longmapsto> B \<^bold>w\<^bold>h\<^bold>e\<^bold>n P)" == "(\<^bold>c\<^bold>a\<^bold>s\<^bold>t A \<longmapsto> B \<^bold>w\<^bold>i\<^bold>t\<^bold>h CONST True \<^bold>w\<^bold>h\<^bold>e\<^bold>n P)"
+definition Cast :: " 'a set \<Rightarrow> 'a set \<Rightarrow> bool \<Rightarrow> bool " ("(2\<^bold>c\<^bold>a\<^bold>s\<^bold>t _ \<longmapsto> _/ \<^bold>w\<^bold>i\<^bold>t\<^bold>h _)" [13,13,13] 12)
+  where "(\<^bold>c\<^bold>a\<^bold>s\<^bold>t A \<longmapsto> B \<^bold>w\<^bold>i\<^bold>t\<^bold>h P) \<longleftrightarrow> (\<forall>v. v \<in> A \<longrightarrow> v \<in> B \<and> P)"
+consts SimpleCast :: " 'a set \<Rightarrow> 'a set \<Rightarrow> bool \<Rightarrow> bool " ("(2\<^bold>c\<^bold>a\<^bold>s\<^bold>t _/ \<longmapsto> _)" [13,13] 12)
+translations "(\<^bold>c\<^bold>a\<^bold>s\<^bold>t A \<longmapsto> B)" == "(\<^bold>c\<^bold>a\<^bold>s\<^bold>t A \<longmapsto> B \<^bold>w\<^bold>i\<^bold>t\<^bold>h CONST True)"
 
-definition CastDual :: " 'a set \<Rightarrow> 'a set \<Rightarrow> bool \<Rightarrow> 'b set \<Rightarrow> 'b set \<Rightarrow> bool \<Rightarrow> bool " ("(2\<^bold>c\<^bold>a\<^bold>s\<^bold>t _/ \<longmapsto> _/ \<^bold>w\<^bold>i\<^bold>t\<^bold>h _/ \<^bold>d\<^bold>u\<^bold>a\<^bold>l _/ \<longmapsto> _/ \<^bold>w\<^bold>h\<^bold>e\<^bold>n _)" [13,13,13,13,13] 12)
-  where "CastDual A B P A' B' Q' \<longleftrightarrow> (\<^bold>d\<^bold>e\<^bold>s\<^bold>t \<^bold>c\<^bold>a\<^bold>s\<^bold>t A \<longmapsto> B \<^bold>w\<^bold>i\<^bold>t\<^bold>h P) \<and> (\<^bold>i\<^bold>n\<^bold>t\<^bold>r\<^bold>o \<^bold>c\<^bold>a\<^bold>s\<^bold>t A' \<longmapsto> B' \<^bold>w\<^bold>h\<^bold>e\<^bold>n Q')"
-consts SimpCastDual1 :: " 'a set \<Rightarrow> 'a set \<Rightarrow> 'b set \<Rightarrow> 'b set \<Rightarrow> bool \<Rightarrow> bool " ("(2\<^bold>c\<^bold>a\<^bold>s\<^bold>t _/ \<longmapsto> _/ \<^bold>d\<^bold>u\<^bold>a\<^bold>l _/ \<longmapsto> _/ \<^bold>w\<^bold>h\<^bold>e\<^bold>n _)" [13,13,13,13] 12)
-consts SimpCastDual2 :: " 'a set \<Rightarrow> 'a set \<Rightarrow> bool \<Rightarrow> 'b set \<Rightarrow> 'b set \<Rightarrow> bool " ("(2\<^bold>c\<^bold>a\<^bold>s\<^bold>t _/ \<longmapsto> _/ \<^bold>w\<^bold>i\<^bold>t\<^bold>h _/ \<^bold>d\<^bold>u\<^bold>a\<^bold>l _/ \<longmapsto> _)" [13,13,13,13] 12)
-consts SimpCastDual3 :: " 'a set \<Rightarrow> 'a set \<Rightarrow> 'b set \<Rightarrow> 'b set \<Rightarrow> bool " ("(2\<^bold>c\<^bold>a\<^bold>s\<^bold>t _/ \<longmapsto> _/ \<^bold>d\<^bold>u\<^bold>a\<^bold>l _/ \<longmapsto> _)" [13,13,13] 12)
+definition CastDual :: " 'a set \<Rightarrow> 'a set \<Rightarrow> bool \<Rightarrow> 'b set \<Rightarrow> 'b set \<Rightarrow> bool " ("(2\<^bold>c\<^bold>a\<^bold>s\<^bold>t _/ \<longmapsto> _/ \<^bold>w\<^bold>i\<^bold>t\<^bold>h _/ \<^bold>d\<^bold>u\<^bold>a\<^bold>l _/ \<longmapsto> _)" [13,13,13,13] 12)
+  where "CastDual A B P A' B' \<longleftrightarrow> (\<forall>v. v \<in> A \<longrightarrow> v \<in> B \<and> P \<and> (\<forall>u. u \<in> A' \<longrightarrow> u \<in> B'))"
+  \<comment> \<open>Intuitively, \<^term>\<open>CastDual A B P A' B' \<longleftrightarrow> (\<^bold>d\<^bold>e\<^bold>s\<^bold>t \<^bold>c\<^bold>a\<^bold>s\<^bold>t A \<longmapsto> B \<^bold>w\<^bold>i\<^bold>t\<^bold>h P) \<and> (Inhabited A \<longrightarrow> (\<^bold>i\<^bold>n\<^bold>t\<^bold>r\<^bold>o \<^bold>c\<^bold>a\<^bold>s\<^bold>t A' \<longmapsto> B'))\<close>\<close>
+
+consts SimpCastDual :: " 'a set \<Rightarrow> 'a set \<Rightarrow> 'b set \<Rightarrow> 'b set \<Rightarrow> bool " ("(2\<^bold>c\<^bold>a\<^bold>s\<^bold>t _/ \<longmapsto> _/ \<^bold>d\<^bold>u\<^bold>a\<^bold>l _/ \<longmapsto> _)" [13,13,13] 12)
 translations
-  "\<^bold>c\<^bold>a\<^bold>s\<^bold>t A \<longmapsto> A' \<^bold>d\<^bold>u\<^bold>a\<^bold>l B \<longmapsto> B'" == "\<^bold>c\<^bold>a\<^bold>s\<^bold>t A \<longmapsto> A' \<^bold>w\<^bold>i\<^bold>t\<^bold>h CONST True \<^bold>d\<^bold>u\<^bold>a\<^bold>l B \<longmapsto> B' \<^bold>w\<^bold>h\<^bold>e\<^bold>n CONST True"
-  "\<^bold>c\<^bold>a\<^bold>s\<^bold>t A \<longmapsto> A' \<^bold>d\<^bold>u\<^bold>a\<^bold>l B \<longmapsto> B' \<^bold>w\<^bold>h\<^bold>e\<^bold>n Q" == "\<^bold>c\<^bold>a\<^bold>s\<^bold>t A \<longmapsto> A' \<^bold>w\<^bold>i\<^bold>t\<^bold>h CONST True \<^bold>d\<^bold>u\<^bold>a\<^bold>l B \<longmapsto> B' \<^bold>w\<^bold>h\<^bold>e\<^bold>n Q"
-  "\<^bold>c\<^bold>a\<^bold>s\<^bold>t A \<longmapsto> A' \<^bold>w\<^bold>i\<^bold>t\<^bold>h P \<^bold>d\<^bold>u\<^bold>a\<^bold>l B \<longmapsto> B'" == "\<^bold>c\<^bold>a\<^bold>s\<^bold>t A \<longmapsto> A' \<^bold>w\<^bold>i\<^bold>t\<^bold>h P \<^bold>d\<^bold>u\<^bold>a\<^bold>l B \<longmapsto> B' \<^bold>w\<^bold>h\<^bold>e\<^bold>n CONST True"
+  "\<^bold>c\<^bold>a\<^bold>s\<^bold>t A \<longmapsto> A' \<^bold>d\<^bold>u\<^bold>a\<^bold>l B \<longmapsto> B'" == "\<^bold>c\<^bold>a\<^bold>s\<^bold>t A \<longmapsto> A' \<^bold>w\<^bold>i\<^bold>t\<^bold>h CONST True \<^bold>d\<^bold>u\<^bold>a\<^bold>l B \<longmapsto> B'"
 
 translations
-  "\<^bold>c\<^bold>a\<^bold>s\<^bold>t x \<tycolon> X \<longmapsto> B \<^bold>w\<^bold>i\<^bold>t\<^bold>h P \<^bold>w\<^bold>h\<^bold>e\<^bold>n Q" == "\<^bold>c\<^bold>a\<^bold>s\<^bold>t \<tort_lbrace> x \<tycolon> X \<tort_rbrace> \<longmapsto> B \<^bold>w\<^bold>i\<^bold>t\<^bold>h P \<^bold>w\<^bold>h\<^bold>e\<^bold>n Q"
-  "\<^bold>c\<^bold>a\<^bold>s\<^bold>t A \<longmapsto> x \<tycolon> X \<^bold>w\<^bold>i\<^bold>t\<^bold>h P \<^bold>w\<^bold>h\<^bold>e\<^bold>n Q" == "\<^bold>c\<^bold>a\<^bold>s\<^bold>t A \<longmapsto> \<tort_lbrace> x \<tycolon> X \<tort_rbrace> \<^bold>w\<^bold>i\<^bold>t\<^bold>h P \<^bold>w\<^bold>h\<^bold>e\<^bold>n Q"
-  "\<^bold>c\<^bold>a\<^bold>s\<^bold>t A \<longmapsto> x \<tycolon> X \<^bold>w\<^bold>i\<^bold>t\<^bold>h P' \<^bold>d\<^bold>u\<^bold>a\<^bold>l A' \<longmapsto> B' \<^bold>w\<^bold>h\<^bold>e\<^bold>n P" == "\<^bold>c\<^bold>a\<^bold>s\<^bold>t A \<longmapsto> \<tort_lbrace>x \<tycolon> X\<tort_rbrace> \<^bold>w\<^bold>i\<^bold>t\<^bold>h P' \<^bold>d\<^bold>u\<^bold>a\<^bold>l A' \<longmapsto> B' \<^bold>w\<^bold>h\<^bold>e\<^bold>n P"
-  "\<^bold>c\<^bold>a\<^bold>s\<^bold>t a \<tycolon> A \<longmapsto> B \<^bold>w\<^bold>i\<^bold>t\<^bold>h P' \<^bold>d\<^bold>u\<^bold>a\<^bold>l A' \<longmapsto> B' \<^bold>w\<^bold>h\<^bold>e\<^bold>n P" == "\<^bold>c\<^bold>a\<^bold>s\<^bold>t \<tort_lbrace>a \<tycolon> A\<tort_rbrace> \<longmapsto> B \<^bold>w\<^bold>i\<^bold>t\<^bold>h P' \<^bold>d\<^bold>u\<^bold>a\<^bold>l A' \<longmapsto> B' \<^bold>w\<^bold>h\<^bold>e\<^bold>n P"
-  "\<^bold>c\<^bold>a\<^bold>s\<^bold>t A \<longmapsto> B \<^bold>w\<^bold>i\<^bold>t\<^bold>h P' \<^bold>d\<^bold>u\<^bold>a\<^bold>l a' \<tycolon> A' \<longmapsto> B' \<^bold>w\<^bold>h\<^bold>e\<^bold>n P" == "\<^bold>c\<^bold>a\<^bold>s\<^bold>t A \<longmapsto> B \<^bold>w\<^bold>i\<^bold>t\<^bold>h P' \<^bold>d\<^bold>u\<^bold>a\<^bold>l \<tort_lbrace>a' \<tycolon> A'\<tort_rbrace> \<longmapsto> B' \<^bold>w\<^bold>h\<^bold>e\<^bold>n P"
-  "\<^bold>c\<^bold>a\<^bold>s\<^bold>t A \<longmapsto> B \<^bold>w\<^bold>i\<^bold>t\<^bold>h P' \<^bold>d\<^bold>u\<^bold>a\<^bold>l A' \<longmapsto> b' \<tycolon> B' \<^bold>w\<^bold>h\<^bold>e\<^bold>n P" == "\<^bold>c\<^bold>a\<^bold>s\<^bold>t A \<longmapsto> B \<^bold>w\<^bold>i\<^bold>t\<^bold>h P' \<^bold>d\<^bold>u\<^bold>a\<^bold>l A' \<longmapsto> \<tort_lbrace>b' \<tycolon> B'\<tort_rbrace> \<^bold>w\<^bold>h\<^bold>e\<^bold>n P"
+  "\<^bold>c\<^bold>a\<^bold>s\<^bold>t x \<tycolon> X \<longmapsto> B \<^bold>w\<^bold>i\<^bold>t\<^bold>h P" == "\<^bold>c\<^bold>a\<^bold>s\<^bold>t \<tort_lbrace> x \<tycolon> X \<tort_rbrace> \<longmapsto> B \<^bold>w\<^bold>i\<^bold>t\<^bold>h P"
+  "\<^bold>c\<^bold>a\<^bold>s\<^bold>t A \<longmapsto> x \<tycolon> X \<^bold>w\<^bold>i\<^bold>t\<^bold>h P" == "\<^bold>c\<^bold>a\<^bold>s\<^bold>t A \<longmapsto> \<tort_lbrace> x \<tycolon> X \<tort_rbrace> \<^bold>w\<^bold>i\<^bold>t\<^bold>h P"
+  "\<^bold>c\<^bold>a\<^bold>s\<^bold>t A \<longmapsto> x \<tycolon> X \<^bold>w\<^bold>i\<^bold>t\<^bold>h P' \<^bold>d\<^bold>u\<^bold>a\<^bold>l A' \<longmapsto> B'" == "\<^bold>c\<^bold>a\<^bold>s\<^bold>t A \<longmapsto> \<tort_lbrace>x \<tycolon> X\<tort_rbrace> \<^bold>w\<^bold>i\<^bold>t\<^bold>h P' \<^bold>d\<^bold>u\<^bold>a\<^bold>l A' \<longmapsto> B'"
+  "\<^bold>c\<^bold>a\<^bold>s\<^bold>t a \<tycolon> A \<longmapsto> B \<^bold>w\<^bold>i\<^bold>t\<^bold>h P' \<^bold>d\<^bold>u\<^bold>a\<^bold>l A' \<longmapsto> B'" == "\<^bold>c\<^bold>a\<^bold>s\<^bold>t \<tort_lbrace>a \<tycolon> A\<tort_rbrace> \<longmapsto> B \<^bold>w\<^bold>i\<^bold>t\<^bold>h P' \<^bold>d\<^bold>u\<^bold>a\<^bold>l A' \<longmapsto> B'"
+  "\<^bold>c\<^bold>a\<^bold>s\<^bold>t A \<longmapsto> B \<^bold>w\<^bold>i\<^bold>t\<^bold>h P' \<^bold>d\<^bold>u\<^bold>a\<^bold>l a' \<tycolon> A' \<longmapsto> B'" == "\<^bold>c\<^bold>a\<^bold>s\<^bold>t A \<longmapsto> B \<^bold>w\<^bold>i\<^bold>t\<^bold>h P' \<^bold>d\<^bold>u\<^bold>a\<^bold>l \<tort_lbrace>a' \<tycolon> A'\<tort_rbrace> \<longmapsto> B'"
+  "\<^bold>c\<^bold>a\<^bold>s\<^bold>t A \<longmapsto> B \<^bold>w\<^bold>i\<^bold>t\<^bold>h P' \<^bold>d\<^bold>u\<^bold>a\<^bold>l A' \<longmapsto> b' \<tycolon> B'" == "\<^bold>c\<^bold>a\<^bold>s\<^bold>t A \<longmapsto> B \<^bold>w\<^bold>i\<^bold>t\<^bold>h P' \<^bold>d\<^bold>u\<^bold>a\<^bold>l A' \<longmapsto> \<tort_lbrace>b' \<tycolon> B'\<tort_rbrace>"
 
 lemma cast_id[\<nu>intro0]: "\<^bold>c\<^bold>a\<^bold>s\<^bold>t A \<longmapsto> A" unfolding Cast_def by fast
 lemma cast_dual_id[\<nu>intro0]: "\<^bold>c\<^bold>a\<^bold>s\<^bold>t A \<longmapsto> A \<^bold>d\<^bold>u\<^bold>a\<^bold>l B \<longmapsto> B"
   unfolding CastDual_def Intro_def Dest_def by (simp add: cast_id)
+
 
 text \<open>There are 3 kinds of the Cast, corresponding 3 usages where the prefix `some_`
 means the variable *can* be schematic (which is unknown in the reasoning) while other variables
@@ -157,10 +151,13 @@ Actually, to prevent reasoning loop all the `dest cast` must constitute a DAG in
   while `intro cast` is that of construction.
 \<close>
 
-lemma [\<nu>intro']: "\<^bold>d\<^bold>e\<^bold>s\<^bold>t \<^bold>c\<^bold>a\<^bold>s\<^bold>t A \<longmapsto> A' \<^bold>w\<^bold>i\<^bold>t\<^bold>h P1 \<Longrightarrow> \<^bold>c\<^bold>a\<^bold>s\<^bold>t A' \<longmapsto> B \<^bold>w\<^bold>i\<^bold>t\<^bold>h P2 \<^bold>w\<^bold>h\<^bold>e\<^bold>n Q \<Longrightarrow> \<^bold>c\<^bold>a\<^bold>s\<^bold>t A \<longmapsto> B \<^bold>w\<^bold>i\<^bold>t\<^bold>h P1 \<and> P2 \<^bold>w\<^bold>h\<^bold>e\<^bold>n Q"
-  unfolding Dest_def Cast_def by auto
-lemma [\<nu>intro']: "\<^bold>i\<^bold>n\<^bold>t\<^bold>r\<^bold>o \<^bold>c\<^bold>a\<^bold>s\<^bold>t B' \<longmapsto> B \<^bold>w\<^bold>h\<^bold>e\<^bold>n Q1 \<Longrightarrow> \<^bold>c\<^bold>a\<^bold>s\<^bold>t A \<longmapsto> B' \<^bold>w\<^bold>i\<^bold>t\<^bold>h P \<^bold>w\<^bold>h\<^bold>e\<^bold>n Q2 \<Longrightarrow> \<^bold>c\<^bold>a\<^bold>s\<^bold>t A \<longmapsto> B \<^bold>w\<^bold>i\<^bold>t\<^bold>h P \<^bold>w\<^bold>h\<^bold>e\<^bold>n Q1 \<and> Q2"
+lemma [\<nu>intro']: "\<^bold>i\<^bold>n\<^bold>t\<^bold>r\<^bold>o \<^bold>c\<^bold>a\<^bold>s\<^bold>t B' \<longmapsto> B \<^bold>w\<^bold>i\<^bold>t\<^bold>h Any \<Longrightarrow> \<^bold>c\<^bold>a\<^bold>s\<^bold>t A \<longmapsto> B' \<^bold>w\<^bold>i\<^bold>t\<^bold>h P \<Longrightarrow> \<^bold>c\<^bold>a\<^bold>s\<^bold>t A \<longmapsto> B \<^bold>w\<^bold>i\<^bold>t\<^bold>h P"
   unfolding Intro_def Cast_def by auto
+lemma [\<nu>intro']: "\<^bold>d\<^bold>e\<^bold>s\<^bold>t \<^bold>c\<^bold>a\<^bold>s\<^bold>t A \<longmapsto> A' \<^bold>w\<^bold>i\<^bold>t\<^bold>h P1 \<Longrightarrow> (P1 \<Longrightarrow> \<^bold>c\<^bold>a\<^bold>s\<^bold>t A' \<longmapsto> B \<^bold>w\<^bold>i\<^bold>t\<^bold>h P2) \<Longrightarrow> \<^bold>c\<^bold>a\<^bold>s\<^bold>t A \<longmapsto> B \<^bold>w\<^bold>i\<^bold>t\<^bold>h P1 \<and> P2"
+  unfolding Dest_def Cast_def by auto
+
+lemma [\<nu>intro'']: "\<^bold>c\<^bold>a\<^bold>s\<^bold>t A \<longmapsto> A' \<^bold>w\<^bold>i\<^bold>t\<^bold>h P \<Longrightarrow> \<^bold>c\<^bold>a\<^bold>s\<^bold>t A \<longmapsto> A' \<^bold>w\<^bold>i\<^bold>t\<^bold>h P \<^bold>d\<^bold>u\<^bold>a\<^bold>l C \<longmapsto> C"
+  unfolding Cast_def CastDual_def Premise_def Dest_def Intro_def by simp
 
 
 (* abbreviation SimpleCast :: " 'a set \<Rightarrow> 'a set \<Rightarrow> bool " ("(2\<^bold>c\<^bold>a\<^bold>s\<^bold>t _ \<longmapsto> _)" [2,14] 13)
@@ -174,8 +171,13 @@ lemma "=_\<nu>cast": "\<^bold>p\<^bold>a\<^bold>r\<^bold>a\<^bold>m x' \<Longrig
 lemma [\<nu>intro']: "\<^bold>p\<^bold>r\<^bold>e\<^bold>m\<^bold>i\<^bold>s\<^bold>e N = N' \<Longrightarrow> \<^bold>p\<^bold>r\<^bold>e\<^bold>m\<^bold>i\<^bold>s\<^bold>e x = x' \<Longrightarrow> \<^bold>c\<^bold>a\<^bold>s\<^bold>t x \<tycolon> N \<longmapsto> x' \<tycolon> N'" unfolding Cast_def Premise_def by simp
 lemma [\<nu>intro0]: "\<^bold>p\<^bold>r\<^bold>e\<^bold>m\<^bold>i\<^bold>s\<^bold>e x = x" unfolding Premise_def by simp
 
-lemma cast_trans: "\<^bold>c\<^bold>a\<^bold>s\<^bold>t A \<longmapsto> B \<^bold>w\<^bold>i\<^bold>t\<^bold>h P \<Longrightarrow> \<^bold>c\<^bold>a\<^bold>s\<^bold>t B \<longmapsto> C \<^bold>w\<^bold>i\<^bold>t\<^bold>h Q \<Longrightarrow> \<^bold>c\<^bold>a\<^bold>s\<^bold>t A \<longmapsto> C \<^bold>w\<^bold>i\<^bold>t\<^bold>h P \<and> Q"
+lemma cast_trans: "\<^bold>c\<^bold>a\<^bold>s\<^bold>t A \<longmapsto> B \<^bold>w\<^bold>i\<^bold>t\<^bold>h P \<Longrightarrow> (P \<Longrightarrow> \<^bold>c\<^bold>a\<^bold>s\<^bold>t B \<longmapsto> C \<^bold>w\<^bold>i\<^bold>t\<^bold>h Q) \<Longrightarrow> \<^bold>c\<^bold>a\<^bold>s\<^bold>t A \<longmapsto> C \<^bold>w\<^bold>i\<^bold>t\<^bold>h P \<and> Q"
   unfolding Cast_def by auto
+lemma cast_dual_trans: 
+  "\<^bold>c\<^bold>a\<^bold>s\<^bold>t A \<longmapsto> B \<^bold>w\<^bold>i\<^bold>t\<^bold>h P1 \<^bold>d\<^bold>u\<^bold>a\<^bold>l B' \<longmapsto> A' \<Longrightarrow> (P1 \<Longrightarrow> \<^bold>c\<^bold>a\<^bold>s\<^bold>t B \<longmapsto> C \<^bold>w\<^bold>i\<^bold>t\<^bold>h P2 \<^bold>d\<^bold>u\<^bold>a\<^bold>l C' \<longmapsto> B')
+    \<Longrightarrow> \<^bold>c\<^bold>a\<^bold>s\<^bold>t A \<longmapsto> C \<^bold>w\<^bold>i\<^bold>t\<^bold>h P1 \<and> P2 \<^bold>d\<^bold>u\<^bold>a\<^bold>l C' \<longmapsto> A'"
+  unfolding Cast_def CastDual_def Intro_def Dest_def by auto
+
 (* lemma dual_cast_fallback[\<nu>intro']: "\<^bold>c\<^bold>a\<^bold>s\<^bold>t A \<longmapsto> B \<^bold>w\<^bold>i\<^bold>t\<^bold>h P \<Longrightarrow> (\<^bold>c\<^bold>a\<^bold>s\<^bold>t A \<longmapsto> B) \<and> (\<^bold>c\<^bold>a\<^bold>s\<^bold>t C \<longmapsto> C)" unfolding Cast_def by fast *)
 
 subsection \<open>Name tag\<close>
@@ -285,6 +287,23 @@ lemma [elim!,\<nu>elim]: "Inhabited \<tort_lbrace>a \<tycolon> A \<heavy_asteris
 
 subsection \<open>Fusion and its derivatives\<close>
 
+subsection \<open>Top Context\<close> \<comment> \<open>The pair of heap and stack\<close>
+
+definition NuTopCtx :: " (heap, 'hx) \<nu> \<Rightarrow> ('s :: stack, 'sx) \<nu> \<Rightarrow> (heap \<times> 's, 'hx \<times> 'sx) \<nu> " (infix "<top-ctx>" 59)
+  where "(H <top-ctx> S) = (\<lambda>(h,s). {(hp,sp). (hp \<nuLinkL> H \<nuLinkR> h) \<and> (sp \<nuLinkL> S \<nuLinkR> s) \<and> Heap hp})"
+consts "NuTopCtx_sugar" :: " 'just \<Rightarrow> 'a \<Rightarrow> 'sugar " ( "(2_ \<heavy_comma>/ \<^bold>h\<^bold>e\<^bold>a\<^bold>p _)" [10,14] 13)
+translations "(s \<tycolon> S\<heavy_comma> \<^bold>h\<^bold>e\<^bold>a\<^bold>p h \<tycolon> H)" \<rightleftharpoons> "(CONST Pair h s) \<tycolon> CONST NuTopCtx H S"
+  "(S\<heavy_comma> \<^bold>h\<^bold>e\<^bold>a\<^bold>p H)" => "(_\<nu>typing_x H, _\<nu>typing_x S) \<tycolon> CONST NuTopCtx (_\<nu>typing_ty H) (_\<nu>typing_ty S)"
+
+lemma [simp]: " ((hp, sp) \<nuLinkL> H <top-ctx> S  \<nuLinkR> (h, s)) \<longleftrightarrow> (hp \<nuLinkL> H  \<nuLinkR> h) \<and> (sp \<nuLinkL> S  \<nuLinkR> s) \<and> Heap hp"
+  unfolding NuTopCtx_def Refining_def by simp
+lemma [elim!,\<nu>elim]: "Inhabited \<tort_lbrace>s \<tycolon> S \<heavy_comma> \<^bold>h\<^bold>e\<^bold>a\<^bold>p h \<tycolon> H\<tort_rbrace> \<Longrightarrow> (s \<ratio> S \<Longrightarrow> h \<ratio> H \<Longrightarrow> C) \<Longrightarrow> C" unfolding Inhabited_def by auto
+
+lemma [\<nu>intro]: "\<^bold>c\<^bold>a\<^bold>s\<^bold>t h \<tycolon> H \<longmapsto> h' \<tycolon> H' \<^bold>w\<^bold>i\<^bold>t\<^bold>h Ph \<Longrightarrow>
+  \<^bold>c\<^bold>a\<^bold>s\<^bold>t s \<tycolon> S \<longmapsto> s' \<tycolon> S' \<^bold>w\<^bold>i\<^bold>t\<^bold>h Ps \<Longrightarrow>
+  \<^bold>c\<^bold>a\<^bold>s\<^bold>t (s \<tycolon> S\<heavy_comma> \<^bold>h\<^bold>e\<^bold>a\<^bold>p h \<tycolon> H) \<longmapsto> (s' \<tycolon> S'\<heavy_comma> \<^bold>h\<^bold>e\<^bold>a\<^bold>p h' \<tycolon> H') \<^bold>w\<^bold>i\<^bold>t\<^bold>h Ph \<and> Ps"
+  unfolding Cast_def by simp blast
+
 subsubsection \<open>Fusion\<close>
 
 definition Fusion :: "('a1,'b1) \<nu> \<Rightarrow> ('a2,'b2) \<nu> \<Rightarrow> ('a1 \<times> 'a2, 'b1 \<times> 'b2) \<nu>" (infixr "\<cross_product>" 70) 
@@ -297,8 +316,8 @@ lemma [elim,\<nu>elim]: "(x1,x2) \<ratio> N1 \<cross_product> N2 \<Longrightarro
 
 lemma [\<nu>intro]: "\<nu>Zero N z1 \<Longrightarrow> \<nu>Zero M z2 \<Longrightarrow> \<nu>Zero (N \<cross_product> M) (z1,z2)" unfolding \<nu>Zero_def by simp
 
-lemma [\<nu>intro]: "\<^bold>c\<^bold>a\<^bold>s\<^bold>t x \<tycolon> N \<longmapsto> x' \<tycolon> N' \<^bold>w\<^bold>i\<^bold>t\<^bold>h P1 \<^bold>w\<^bold>h\<^bold>e\<^bold>n Q1 \<Longrightarrow> \<^bold>c\<^bold>a\<^bold>s\<^bold>t y \<tycolon> M \<longmapsto> y' \<tycolon> M' \<^bold>w\<^bold>i\<^bold>t\<^bold>h P2 \<^bold>w\<^bold>h\<^bold>e\<^bold>n Q2 \<Longrightarrow>
-  \<^bold>c\<^bold>a\<^bold>s\<^bold>t (x,y) \<tycolon> N \<cross_product> M \<longmapsto> (x',y') \<tycolon> N' \<cross_product> M' \<^bold>w\<^bold>i\<^bold>t\<^bold>h P1 \<and> P2 \<^bold>w\<^bold>h\<^bold>e\<^bold>n Q1 \<and> Q2" unfolding Cast_def by simp blast
+lemma [\<nu>intro]: "\<^bold>c\<^bold>a\<^bold>s\<^bold>t x \<tycolon> N \<longmapsto> x' \<tycolon> N' \<^bold>w\<^bold>i\<^bold>t\<^bold>h P1 \<Longrightarrow> \<^bold>c\<^bold>a\<^bold>s\<^bold>t y \<tycolon> M \<longmapsto> y' \<tycolon> M' \<^bold>w\<^bold>i\<^bold>t\<^bold>h P2 \<Longrightarrow>
+  \<^bold>c\<^bold>a\<^bold>s\<^bold>t (x,y) \<tycolon> N \<cross_product> M \<longmapsto> (x',y') \<tycolon> N' \<cross_product> M' \<^bold>w\<^bold>i\<^bold>t\<^bold>h P1 \<and> P2" unfolding Cast_def by simp blast
 
 (* no_notation RepSet ("\<tort_lbrace> _ \<tort_rbrace>" [10] )
 syntax "_RepSet" :: "\<nu>typing \<Rightarrow> 'a set"  ("\<tort_lbrace> _ \<tort_rbrace>" [10] )
@@ -315,28 +334,42 @@ translations " a \<tycolon> A\<heavy_comma> b \<tycolon> B " == " (CONST Pair b 
 
 lemma [simp]: "(pa,pb) \<nuLinkL> A <stack-div> B \<nuLinkR> (xa,xb) \<longleftrightarrow> (pa \<nuLinkL> A \<nuLinkR> xa) \<and> (pb \<nuLinkL> B \<nuLinkR> xb)" unfolding Stack_Delimiter_def by simp
 
-lemma [\<nu>intro]: "\<^bold>c\<^bold>a\<^bold>s\<^bold>t a \<tycolon> A \<longmapsto> a' \<tycolon> A' \<^bold>w\<^bold>i\<^bold>t\<^bold>h P1 \<^bold>w\<^bold>h\<^bold>e\<^bold>n Q1 \<Longrightarrow> \<^bold>c\<^bold>a\<^bold>s\<^bold>t b \<tycolon> B \<longmapsto> b' \<tycolon> B' \<^bold>w\<^bold>i\<^bold>t\<^bold>h P2 \<^bold>w\<^bold>h\<^bold>e\<^bold>n Q2 \<Longrightarrow>
-  \<^bold>c\<^bold>a\<^bold>s\<^bold>t (a \<tycolon> A\<heavy_comma> b \<tycolon> B) \<longmapsto> (a' \<tycolon> A'\<heavy_comma> b' \<tycolon> B') \<^bold>w\<^bold>i\<^bold>t\<^bold>h P1 \<and> P2 \<^bold>w\<^bold>h\<^bold>e\<^bold>n Q1 \<and> Q2"
+lemma [\<nu>intro]: "\<^bold>c\<^bold>a\<^bold>s\<^bold>t a \<tycolon> A \<longmapsto> a' \<tycolon> A' \<^bold>w\<^bold>i\<^bold>t\<^bold>h P1 \<Longrightarrow> (P1 \<Longrightarrow> \<^bold>c\<^bold>a\<^bold>s\<^bold>t b \<tycolon> B \<longmapsto> b' \<tycolon> B' \<^bold>w\<^bold>i\<^bold>t\<^bold>h P2) \<Longrightarrow>
+  \<^bold>c\<^bold>a\<^bold>s\<^bold>t (a \<tycolon> A\<heavy_comma> b \<tycolon> B) \<longmapsto> (a' \<tycolon> A'\<heavy_comma> b' \<tycolon> B') \<^bold>w\<^bold>i\<^bold>t\<^bold>h P1 \<and> P2"
   unfolding Cast_def by simp blast
 
-subsection \<open>Top Context\<close>
+subsubsection \<open>Front Stack\<close>
 
-subsubsection \<open>Context Type\<close> \<comment> \<open>The pair of heap and stack\<close>
+definition Nu_Front_Stack :: "('a::lrep,'ax) \<nu> \<Rightarrow> (heap \<times> 'stack,'hsx) \<nu> \<Rightarrow> (heap \<times> 'a \<times> 'stack, 'ax \<times> 'hsx) \<nu>"
+  where "Nu_Front_Stack A Ctx = (\<lambda>(ax,hsx). {(h,a,s). (a \<nuLinkL> A \<nuLinkR> ax) \<and> ((h,s) \<nuLinkL> Ctx \<nuLinkR> (hsx))} )"
 
-definition NuTopCtx :: " (heap, 'hx) \<nu> \<Rightarrow> ('s :: stack, 'sx) \<nu> \<Rightarrow> (heap \<times> 's, 'hx \<times> 'sx) \<nu> " (infix "<top-ctx>" 59)
-  where "(H <top-ctx> S) = (\<lambda>(h,s). {(hp,sp). (hp \<nuLinkL> H \<nuLinkR> h) \<and> (sp \<nuLinkL> S \<nuLinkR> s) \<and> Heap hp})"
-consts "NuTopCtx_sugar" :: " 'just \<Rightarrow> 'a \<Rightarrow> 'sugar " ( "(2_ \<heavy_comma>/ \<^bold>h\<^bold>e\<^bold>a\<^bold>p _)" [10,14] 13)
-translations "(s \<tycolon> S\<heavy_comma> \<^bold>h\<^bold>e\<^bold>a\<^bold>p h \<tycolon> H)" \<rightleftharpoons> "(CONST Pair h s) \<tycolon> CONST NuTopCtx H S"
-  "(S\<heavy_comma> \<^bold>h\<^bold>e\<^bold>a\<^bold>p H)" => "(_\<nu>typing_x H, _\<nu>typing_x S) \<tycolon> CONST NuTopCtx (_\<nu>typing_ty H) (_\<nu>typing_ty S)"
+consts "Front_Stack_sugar" :: " 'just \<Rightarrow> 'a \<Rightarrow> 'sugar " ( "_/ \<heavy_comma>^ _" [13,14] 13) \<comment> \<open>Note it is left associative\<close>
+translations " c \<tycolon> Ctx \<heavy_comma>^ a \<tycolon> A " == " (CONST Pair a c) \<tycolon> (CONST Nu_Front_Stack A Ctx) "
+  " Ctx \<heavy_comma>^ A " => " (CONST Pair (_\<nu>typing_x A) (_\<nu>typing_x Ctx)) \<tycolon> (CONST Nu_Front_Stack (_\<nu>typing_ty A) (_\<nu>typing_ty Ctx)) "
 
-lemma [simp]: " ((hp, sp) \<nuLinkL> H <top-ctx> S  \<nuLinkR> (h, s)) \<longleftrightarrow> (hp \<nuLinkL> H  \<nuLinkR> h) \<and> (sp \<nuLinkL> S  \<nuLinkR> s) \<and> Heap hp"
-  unfolding NuTopCtx_def Refining_def by simp
-lemma [elim!,\<nu>elim]: "Inhabited \<tort_lbrace>s \<tycolon> S \<heavy_comma> \<^bold>h\<^bold>e\<^bold>a\<^bold>p h \<tycolon> H\<tort_rbrace> \<Longrightarrow> (s \<ratio> S \<Longrightarrow> h \<ratio> H \<Longrightarrow> C) \<Longrightarrow> C" unfolding Inhabited_def by auto
+text \<open>Normally the stack elements are written `before` the heap elements, \<^term>\<open>s1 \<tycolon> S1\<heavy_comma> s2 \<tycolon> S2\<heavy_comma> \<^bold>h\<^bold>e\<^bold>a\<^bold>p h \<tycolon> H\<close>.
+  The \<^term>\<open>Nu_Front_Stack\<close> allows one writes the stack elements `after` the heap, as \<^term>\<open>s1 \<tycolon> S1\<heavy_comma> \<^bold>h\<^bold>e\<^bold>a\<^bold>p h \<tycolon> H \<heavy_comma>^ s2 \<tycolon> S2\<close>.
+  Both of the two \<nu>-types specify the same low concretes.
+  It is useful when one needs to specify over the whole remaining stack and heap, e.g., theorem `Until` (see later)
+    which requires body to return \<^term>\<open>x \<tycolon> X \<heavy_comma>^ loop_condition \<tycolon> \<bool>\<close> where the \<^term>\<open>x \<tycolon> X\<close> instantiated by caller
+    specifies all the heap and remaining stack except the leading loop_condition.\<close>
 
-lemma [\<nu>intro]: "\<^bold>c\<^bold>a\<^bold>s\<^bold>t h \<tycolon> H \<longmapsto> h' \<tycolon> H' \<^bold>w\<^bold>i\<^bold>t\<^bold>h Ph \<^bold>w\<^bold>h\<^bold>e\<^bold>n Qh \<Longrightarrow>
-  \<^bold>c\<^bold>a\<^bold>s\<^bold>t s \<tycolon> S \<longmapsto> s' \<tycolon> S' \<^bold>w\<^bold>i\<^bold>t\<^bold>h Ps \<^bold>w\<^bold>h\<^bold>e\<^bold>n Qs \<Longrightarrow>
-  \<^bold>c\<^bold>a\<^bold>s\<^bold>t (s \<tycolon> S\<heavy_comma> \<^bold>h\<^bold>e\<^bold>a\<^bold>p h \<tycolon> H) \<longmapsto> (s' \<tycolon> S'\<heavy_comma> \<^bold>h\<^bold>e\<^bold>a\<^bold>p h' \<tycolon> H') \<^bold>w\<^bold>i\<^bold>t\<^bold>h Ph \<and> Ps \<^bold>w\<^bold>h\<^bold>e\<^bold>n Qh \<and> Qs"
-  unfolding Cast_def by simp blast
+lemma [simp]: "(h,a,s) \<nuLinkL> Nu_Front_Stack A Ctx \<nuLinkR> (ax,hsx) \<longleftrightarrow> (a \<nuLinkL> A \<nuLinkR> ax) \<and> ((h,s) \<nuLinkL> Ctx \<nuLinkR> hsx)"
+  unfolding Nu_Front_Stack_def Refining_def by simp
+lemma [simp]: "\<tort_lbrace> (a,h,s) \<tycolon> Nu_Front_Stack A (NuTopCtx H S) \<tort_rbrace> = \<tort_lbrace> (h,a,s) \<tycolon> NuTopCtx H (A <stack-div> S) \<tort_rbrace>" by auto
+
+lemma Nu_Front_Stack_cong: "\<tort_lbrace>c \<tycolon> Ctx\<tort_rbrace> \<equiv> \<tort_lbrace>c' \<tycolon> Ctx'\<tort_rbrace> \<Longrightarrow> \<tort_lbrace>c \<tycolon> Ctx \<heavy_comma>^ x \<tycolon> T\<tort_rbrace> \<equiv> \<tort_lbrace>c' \<tycolon> Ctx' \<heavy_comma>^ x \<tycolon> T\<tort_rbrace>"
+  unfolding atomize_eq by auto
+simproc_setup Nu_Front_Stack_cong ("\<tort_lbrace>c \<tycolon> Ctx \<heavy_comma>^ x \<tycolon> T\<tort_rbrace>") = \<open>K (NuSimpCong.simproc @{thm Nu_Front_Stack_cong})\<close>
+
+lemma [\<nu>intro]: "\<^bold>c\<^bold>a\<^bold>s\<^bold>t R\<heavy_comma> \<^bold>h\<^bold>e\<^bold>a\<^bold>p H \<longmapsto> c \<tycolon> Ctx \<^bold>w\<^bold>i\<^bold>t\<^bold>h P \<Longrightarrow> \<^bold>i\<^bold>n\<^bold>t\<^bold>r\<^bold>o \<^bold>c\<^bold>a\<^bold>s\<^bold>t R\<heavy_comma> x \<tycolon> X\<heavy_comma> \<^bold>h\<^bold>e\<^bold>a\<^bold>p H \<longmapsto> c \<tycolon> Ctx \<heavy_comma>^ (x \<tycolon> X)"
+  unfolding Intro_def Cast_def by simp
+lemma [\<nu>intro]: "\<^bold>c\<^bold>a\<^bold>s\<^bold>t c \<tycolon> Ctx \<longmapsto> (R\<heavy_comma> \<^bold>h\<^bold>e\<^bold>a\<^bold>p H) \<^bold>w\<^bold>i\<^bold>t\<^bold>h P
+    \<Longrightarrow> \<^bold>d\<^bold>e\<^bold>s\<^bold>t \<^bold>c\<^bold>a\<^bold>s\<^bold>t c \<tycolon> Ctx \<heavy_comma>^ (x \<tycolon> X) \<longmapsto> (R\<heavy_comma> x \<tycolon> X\<heavy_comma> \<^bold>h\<^bold>e\<^bold>a\<^bold>p H) \<^bold>w\<^bold>i\<^bold>t\<^bold>h P"
+  unfolding Dest_def Cast_def by simp blast
+
+
+
 
 subsection \<open>Existential Nu-type\<close>
 
@@ -373,11 +406,12 @@ lemma [simp]: "p \<in> \<S>  \<tort_lbrace>x \<tycolon> ExNu T\<tort_rbrace> \<l
 lemma [simp]: "p \<in> \<S_S> \<tort_lbrace>x \<tycolon> ExNu T\<tort_rbrace> \<longleftrightarrow> (\<exists>z. p \<in> \<S_S> \<tort_lbrace>x z \<tycolon> T z\<tort_rbrace>)" by (auto 4 3)
 lemma [simp]: "\<tort_lbrace>x \<tycolon> ExNu T \<heavy_comma> y \<tycolon> R\<tort_rbrace> = \<tort_lbrace>\<exists>* c. x c \<tycolon> T c \<heavy_comma> y \<tycolon> R \<tort_rbrace>" unfolding Stack_Delimiter_def by auto
 lemma [simp]: "\<tort_lbrace>y \<tycolon> L \<heavy_comma> x \<tycolon> ExNu T\<tort_rbrace> = \<tort_lbrace>\<exists>* c. y \<tycolon> L \<heavy_comma> x c \<tycolon> T c \<tort_rbrace>" unfolding Stack_Delimiter_def by auto
+
 lemma ExTyp_strip: "(\<^bold>c\<^bold>u\<^bold>r\<^bold>r\<^bold>e\<^bold>n\<^bold>t p \<^bold>r\<^bold>e\<^bold>s\<^bold>u\<^bold>l\<^bold>t\<^bold>s \<^bold>i\<^bold>n (x \<tycolon> ExNu T)) \<equiv> (\<exists>c. \<^bold>c\<^bold>u\<^bold>r\<^bold>r\<^bold>e\<^bold>n\<^bold>t p \<^bold>r\<^bold>e\<^bold>s\<^bold>u\<^bold>l\<^bold>t\<^bold>s \<^bold>i\<^bold>n x c \<tycolon> T c)"
   unfolding CurrentConstruction_def by auto
 
 lemma [\<nu>intro]: "\<^bold>i\<^bold>n\<^bold>t\<^bold>r\<^bold>o \<^bold>c\<^bold>a\<^bold>s\<^bold>t x c \<tycolon> T c \<longmapsto> (\<exists>*c. x c \<tycolon> T c)" unfolding Intro_def Cast_def by simp blast
-lemma [\<nu>intro]: "(\<And>c. \<^bold>c\<^bold>a\<^bold>s\<^bold>t x c \<tycolon> T c \<longmapsto> x' c \<tycolon> T' c \<^bold>w\<^bold>i\<^bold>t\<^bold>h P c \<^bold>w\<^bold>h\<^bold>e\<^bold>n Q c) \<Longrightarrow> \<^bold>c\<^bold>a\<^bold>s\<^bold>t (\<exists>*c. x c \<tycolon> T c) \<longmapsto> (\<exists>*c. x' c \<tycolon> T' c) \<^bold>w\<^bold>i\<^bold>t\<^bold>h (\<exists>c. P c) \<^bold>w\<^bold>h\<^bold>e\<^bold>n (\<forall>c. Q c)"
+lemma [\<nu>intro]: "(\<And>c. \<^bold>c\<^bold>a\<^bold>s\<^bold>t x c \<tycolon> T c \<longmapsto> x' c \<tycolon> T' c \<^bold>w\<^bold>i\<^bold>t\<^bold>h P c) \<Longrightarrow> \<^bold>c\<^bold>a\<^bold>s\<^bold>t (\<exists>*c. x c \<tycolon> T c) \<longmapsto> (\<exists>*c. x' c \<tycolon> T' c) \<^bold>w\<^bold>i\<^bold>t\<^bold>h (\<exists>c. P c)"
   unfolding Cast_def by auto
 
 
@@ -465,6 +499,7 @@ lemma [simp]: "\<tort_lbrace>L \<heavy_asterisk> (x \<tycolon> T) \<and>\<^sup>\
 lemma [simp]: "\<tort_lbrace> (s \<tycolon> S) \<and>\<^sup>\<nu>\<^sub>a\<^sub>u\<^sub>t\<^sub>o P \<heavy_comma> \<^bold>h\<^bold>e\<^bold>a\<^bold>p h \<tycolon> H \<tort_rbrace> = \<tort_lbrace> (s \<tycolon> S\<heavy_comma> \<^bold>h\<^bold>e\<^bold>a\<^bold>p h \<tycolon> H) \<and>\<^sup>\<nu>\<^sub>a\<^sub>u\<^sub>t\<^sub>o P \<tort_rbrace>"
     and [simp]: "\<tort_lbrace> s \<tycolon> S \<heavy_comma> \<^bold>h\<^bold>e\<^bold>a\<^bold>p (h \<tycolon> H) \<and>\<^sup>\<nu>\<^sub>a\<^sub>u\<^sub>t\<^sub>o P \<tort_rbrace> = \<tort_lbrace> (s \<tycolon> S\<heavy_comma> \<^bold>h\<^bold>e\<^bold>a\<^bold>p h \<tycolon> H) \<and>\<^sup>\<nu>\<^sub>a\<^sub>u\<^sub>t\<^sub>o P \<tort_rbrace>"
   unfolding Auto_def by auto
+lemma [simp]: "\<tort_lbrace>c \<tycolon> Ctx \<and>\<^sup>\<nu>\<^sub>a\<^sub>u\<^sub>t\<^sub>o P \<heavy_comma>^ x \<tycolon> T\<tort_rbrace> = \<tort_lbrace> (c \<tycolon> Ctx \<heavy_comma>^ x \<tycolon> T) \<and>\<^sup>\<nu>\<^sub>a\<^sub>u\<^sub>t\<^sub>o P \<tort_rbrace>" unfolding Auto_def by auto
 
 lemma AutoAddition_cong: "\<tort_lbrace>x \<tycolon> T\<tort_rbrace> \<equiv> \<tort_lbrace>x' \<tycolon> T'\<tort_rbrace> \<Longrightarrow> \<tort_lbrace>x \<tycolon> T \<and>\<^sup>\<nu>\<^sub>a\<^sub>u\<^sub>t\<^sub>o P\<tort_rbrace> \<equiv> \<tort_lbrace>x' \<tycolon> T' \<and>\<^sup>\<nu>\<^sub>a\<^sub>u\<^sub>t\<^sub>o P\<tort_rbrace>" unfolding Auto_def by simp
 simproc_setup AutoAddition_cong ("\<tort_lbrace>x \<tycolon> T \<and>\<^sup>\<nu>\<^sub>a\<^sub>u\<^sub>t\<^sub>o P\<tort_rbrace>") = \<open>K (NuSimpCong.simproc @{thm AutoAddition_cong})\<close>
@@ -553,8 +588,8 @@ lemma context_cast[\<nu>intro]:
 
 lemma context_cast_dual[\<nu>intro]:
   "\<^bold>c\<^bold>a\<^bold>s\<^bold>t k \<tycolon> K \<longmapsto> k' \<tycolon> K' \<^bold>w\<^bold>i\<^bold>t\<^bold>h PK
-    \<Longrightarrow> \<^bold>c\<^bold>a\<^bold>s\<^bold>t h \<tycolon> H \<longmapsto> h' \<tycolon> \<medium_left_bracket> H' \<medium_right_bracket> \<^bold>w\<^bold>i\<^bold>t\<^bold>h PH \<^bold>d\<^bold>u\<^bold>a\<^bold>l h2 \<tycolon> \<medium_left_bracket> H2 \<medium_right_bracket> \<longmapsto> h2' \<tycolon> H2' \<^bold>w\<^bold>h\<^bold>e\<^bold>n QH
-    \<Longrightarrow> \<^bold>c\<^bold>a\<^bold>s\<^bold>t (k \<tycolon> K\<heavy_comma> \<^bold>h\<^bold>e\<^bold>a\<^bold>p h \<tycolon> H) \<longmapsto> (k' \<tycolon> K'\<heavy_comma> \<^bold>h\<^bold>e\<^bold>a\<^bold>p h' \<tycolon> H') \<^bold>w\<^bold>i\<^bold>t\<^bold>h PK \<and> PH \<^bold>d\<^bold>u\<^bold>a\<^bold>l (k2 \<tycolon> K2\<heavy_comma> \<^bold>h\<^bold>e\<^bold>a\<^bold>p h2 \<tycolon> H2) \<longmapsto> (k2 \<tycolon> K2\<heavy_comma> \<^bold>h\<^bold>e\<^bold>a\<^bold>p h2' \<tycolon> H2') \<^bold>w\<^bold>h\<^bold>e\<^bold>n QH"
+    \<Longrightarrow> (PK \<Longrightarrow> \<^bold>c\<^bold>a\<^bold>s\<^bold>t h \<tycolon> H \<longmapsto> h' \<tycolon> \<medium_left_bracket> H' \<medium_right_bracket> \<^bold>w\<^bold>i\<^bold>t\<^bold>h PH \<^bold>d\<^bold>u\<^bold>a\<^bold>l h2 \<tycolon> \<medium_left_bracket> H2 \<medium_right_bracket> \<longmapsto> h2' \<tycolon> H2')
+    \<Longrightarrow> \<^bold>c\<^bold>a\<^bold>s\<^bold>t (k \<tycolon> K\<heavy_comma> \<^bold>h\<^bold>e\<^bold>a\<^bold>p h \<tycolon> H) \<longmapsto> (k' \<tycolon> K'\<heavy_comma> \<^bold>h\<^bold>e\<^bold>a\<^bold>p h' \<tycolon> H') \<^bold>w\<^bold>i\<^bold>t\<^bold>h PK \<and> PH \<^bold>d\<^bold>u\<^bold>a\<^bold>l (k2 \<tycolon> K2\<heavy_comma> \<^bold>h\<^bold>e\<^bold>a\<^bold>p h2 \<tycolon> H2) \<longmapsto> (k2 \<tycolon> K2\<heavy_comma> \<^bold>h\<^bold>e\<^bold>a\<^bold>p h2' \<tycolon> H2')"
   unfolding CastDual_def Cast_def Heap_Cast_Goal_def Intro_def Dest_def by (auto simp add: pair_forall)
 
 (* lemma [\<nu>intro0]: "\<^bold>c\<^bold>a\<^bold>s\<^bold>t x \<tycolon> X \<longmapsto> H' \<heavy_asterisk> y \<tycolon> Y \<^bold>w\<^bold>i\<^bold>t\<^bold>h P \<^bold>d\<^bold>u\<^bold>a\<^bold>l H'\<^sub>m \<heavy_asterisk> y\<^sub>m \<tycolon> Y \<longmapsto> x\<^sub>m \<tycolon> X \<^bold>w\<^bold>h\<^bold>e\<^bold>n Q
@@ -569,28 +604,28 @@ lemma heap_idx_this[\<nu>intro]:
   unfolding Cast_def Separation_emptyL Heap_Cast_Goal_def CastDual_def Intro_def Dest_def by simp
 
 lemma heap_idx_L[\<nu>intro0]:
-  "\<^bold>c\<^bold>a\<^bold>s\<^bold>t h \<tycolon> H \<longmapsto> h' \<tycolon> H' \<heavy_asterisk> x \<tycolon> \<medium_left_bracket> X \<medium_right_bracket> \<^bold>w\<^bold>i\<^bold>t\<^bold>h P \<^bold>d\<^bold>u\<^bold>a\<^bold>l h'\<^sub>m \<tycolon> H'\<^sub>m \<heavy_asterisk> x\<^sub>m \<tycolon> \<medium_left_bracket> X\<^sub>m \<medium_right_bracket> \<longmapsto> h\<^sub>m \<tycolon> H\<^sub>m \<^bold>w\<^bold>h\<^bold>e\<^bold>n Q
-    \<Longrightarrow> \<^bold>c\<^bold>a\<^bold>s\<^bold>t l \<tycolon> L \<heavy_asterisk> h \<tycolon> H \<longmapsto> l \<tycolon> L \<heavy_asterisk> h' \<tycolon> H' \<heavy_asterisk> x \<tycolon> \<medium_left_bracket> X \<medium_right_bracket> \<^bold>w\<^bold>i\<^bold>t\<^bold>h P \<^bold>d\<^bold>u\<^bold>a\<^bold>l l \<tycolon> L \<heavy_asterisk> h'\<^sub>m \<tycolon> H'\<^sub>m \<heavy_asterisk> x\<^sub>m \<tycolon> \<medium_left_bracket> X\<^sub>m \<medium_right_bracket> \<longmapsto> l \<tycolon> L \<heavy_asterisk> h\<^sub>m \<tycolon> H\<^sub>m \<^bold>w\<^bold>h\<^bold>e\<^bold>n Q"
+  "\<^bold>c\<^bold>a\<^bold>s\<^bold>t h \<tycolon> H \<longmapsto> h' \<tycolon> H' \<heavy_asterisk> x \<tycolon> \<medium_left_bracket> X \<medium_right_bracket> \<^bold>w\<^bold>i\<^bold>t\<^bold>h P \<^bold>d\<^bold>u\<^bold>a\<^bold>l h'\<^sub>m \<tycolon> H'\<^sub>m \<heavy_asterisk> x\<^sub>m \<tycolon> \<medium_left_bracket> X\<^sub>m \<medium_right_bracket> \<longmapsto> h\<^sub>m \<tycolon> H\<^sub>m
+    \<Longrightarrow> \<^bold>c\<^bold>a\<^bold>s\<^bold>t l \<tycolon> L \<heavy_asterisk> h \<tycolon> H \<longmapsto> l \<tycolon> L \<heavy_asterisk> h' \<tycolon> H' \<heavy_asterisk> x \<tycolon> \<medium_left_bracket> X \<medium_right_bracket> \<^bold>w\<^bold>i\<^bold>t\<^bold>h P \<^bold>d\<^bold>u\<^bold>a\<^bold>l l \<tycolon> L \<heavy_asterisk> h'\<^sub>m \<tycolon> H'\<^sub>m \<heavy_asterisk> x\<^sub>m \<tycolon> \<medium_left_bracket> X\<^sub>m \<medium_right_bracket> \<longmapsto> l \<tycolon> L \<heavy_asterisk> h\<^sub>m \<tycolon> H\<^sub>m"
   unfolding Cast_def CastDual_def Heap_Cast_Goal_def SepNu_2_SepSet Intro_def Dest_def
   by (smt (verit, del_insts) SeparationSet_assoc SeparationSet_comm SeparationSet_def mem_Collect_eq)
 
 lemma heap_idx_R[\<nu>intro]:
-  "\<^bold>c\<^bold>a\<^bold>s\<^bold>t h \<tycolon> H \<longmapsto> h' \<tycolon> H' \<heavy_asterisk> x \<tycolon> \<medium_left_bracket> X \<medium_right_bracket> \<^bold>w\<^bold>i\<^bold>t\<^bold>h P \<^bold>d\<^bold>u\<^bold>a\<^bold>l h'\<^sub>m \<tycolon> H'\<^sub>m \<heavy_asterisk> x\<^sub>m \<tycolon> \<medium_left_bracket> X\<^sub>m \<medium_right_bracket> \<longmapsto> h\<^sub>m \<tycolon> H\<^sub>m \<^bold>w\<^bold>h\<^bold>e\<^bold>n Q
-    \<Longrightarrow> \<^bold>c\<^bold>a\<^bold>s\<^bold>t h \<tycolon> H \<heavy_asterisk> r \<tycolon> R \<longmapsto> h' \<tycolon> H' \<heavy_asterisk> r \<tycolon> R \<heavy_asterisk> x \<tycolon> \<medium_left_bracket> X \<medium_right_bracket> \<^bold>w\<^bold>i\<^bold>t\<^bold>h P \<^bold>d\<^bold>u\<^bold>a\<^bold>l h'\<^sub>m \<tycolon> H'\<^sub>m \<heavy_asterisk> r \<tycolon> R \<heavy_asterisk> x\<^sub>m \<tycolon> \<medium_left_bracket> X\<^sub>m \<medium_right_bracket> \<longmapsto> h\<^sub>m \<tycolon> H\<^sub>m \<heavy_asterisk> r \<tycolon> \<medium_left_bracket> R \<medium_right_bracket> \<^bold>w\<^bold>h\<^bold>e\<^bold>n Q"
+  "\<^bold>c\<^bold>a\<^bold>s\<^bold>t h \<tycolon> H \<longmapsto> h' \<tycolon> H' \<heavy_asterisk> x \<tycolon> \<medium_left_bracket> X \<medium_right_bracket> \<^bold>w\<^bold>i\<^bold>t\<^bold>h P \<^bold>d\<^bold>u\<^bold>a\<^bold>l h'\<^sub>m \<tycolon> H'\<^sub>m \<heavy_asterisk> x\<^sub>m \<tycolon> \<medium_left_bracket> X\<^sub>m \<medium_right_bracket> \<longmapsto> h\<^sub>m \<tycolon> H\<^sub>m
+    \<Longrightarrow> \<^bold>c\<^bold>a\<^bold>s\<^bold>t h \<tycolon> H \<heavy_asterisk> r \<tycolon> R \<longmapsto> h' \<tycolon> H' \<heavy_asterisk> r \<tycolon> R \<heavy_asterisk> x \<tycolon> \<medium_left_bracket> X \<medium_right_bracket> \<^bold>w\<^bold>i\<^bold>t\<^bold>h P \<^bold>d\<^bold>u\<^bold>a\<^bold>l h'\<^sub>m \<tycolon> H'\<^sub>m \<heavy_asterisk> r \<tycolon> R \<heavy_asterisk> x\<^sub>m \<tycolon> \<medium_left_bracket> X\<^sub>m \<medium_right_bracket> \<longmapsto> h\<^sub>m \<tycolon> H\<^sub>m \<heavy_asterisk> r \<tycolon> \<medium_left_bracket> R \<medium_right_bracket>"
   unfolding Cast_def CastDual_def Heap_Cast_Goal_def SepNu_2_SepSet Intro_def Dest_def
   by (smt (verit, del_insts) SeparationSet_assoc SeparationSet_comm SeparationSet_def mem_Collect_eq)
 
 lemma [\<nu>intro]:
-  "\<^bold>c\<^bold>a\<^bold>s\<^bold>t h \<tycolon> H \<longmapsto> h1 \<tycolon> H1 \<heavy_asterisk> x \<tycolon> \<medium_left_bracket> X \<medium_right_bracket> \<^bold>w\<^bold>i\<^bold>t\<^bold>h P1 \<^bold>d\<^bold>u\<^bold>a\<^bold>l h1\<^sub>m \<tycolon> H1\<^sub>m \<heavy_asterisk> x\<^sub>m \<tycolon> \<medium_left_bracket> X\<^sub>m \<medium_right_bracket> \<longmapsto> h\<^sub>m \<tycolon> H\<^sub>m \<^bold>w\<^bold>h\<^bold>e\<^bold>n Q1
-    \<Longrightarrow> \<^bold>c\<^bold>a\<^bold>s\<^bold>t h1 \<tycolon> H1 \<longmapsto> h2 \<tycolon> \<medium_left_bracket> H2 \<medium_right_bracket> \<^bold>w\<^bold>i\<^bold>t\<^bold>h P2 \<^bold>d\<^bold>u\<^bold>a\<^bold>l h2\<^sub>m \<tycolon> \<medium_left_bracket> H2\<^sub>m \<medium_right_bracket> \<longmapsto> h1\<^sub>m \<tycolon> H1\<^sub>m \<^bold>w\<^bold>h\<^bold>e\<^bold>n Q2
-    \<Longrightarrow> \<^bold>c\<^bold>a\<^bold>s\<^bold>t h \<tycolon> H \<longmapsto> (x, h2) \<tycolon> \<medium_left_bracket> X <heap-sep> H2 \<medium_right_bracket> \<^bold>w\<^bold>i\<^bold>t\<^bold>h P1 \<and> P2 \<^bold>d\<^bold>u\<^bold>a\<^bold>l (x\<^sub>m, h2\<^sub>m) \<tycolon> \<medium_left_bracket> X\<^sub>m <heap-sep> H2\<^sub>m \<medium_right_bracket> \<longmapsto> h\<^sub>m \<tycolon> H\<^sub>m \<^bold>w\<^bold>h\<^bold>e\<^bold>n Q1 \<and> Q2"
+  "\<^bold>c\<^bold>a\<^bold>s\<^bold>t h \<tycolon> H \<longmapsto> h1 \<tycolon> H1 \<heavy_asterisk> x \<tycolon> \<medium_left_bracket> X \<medium_right_bracket> \<^bold>w\<^bold>i\<^bold>t\<^bold>h P1 \<^bold>d\<^bold>u\<^bold>a\<^bold>l h1\<^sub>m \<tycolon> H1\<^sub>m \<heavy_asterisk> x\<^sub>m \<tycolon> \<medium_left_bracket> X\<^sub>m \<medium_right_bracket> \<longmapsto> h\<^sub>m \<tycolon> H\<^sub>m
+    \<Longrightarrow> (P1 \<Longrightarrow> \<^bold>c\<^bold>a\<^bold>s\<^bold>t h1 \<tycolon> H1 \<longmapsto> h2 \<tycolon> \<medium_left_bracket> H2 \<medium_right_bracket> \<^bold>w\<^bold>i\<^bold>t\<^bold>h P2 \<^bold>d\<^bold>u\<^bold>a\<^bold>l h2\<^sub>m \<tycolon> \<medium_left_bracket> H2\<^sub>m \<medium_right_bracket> \<longmapsto> h1\<^sub>m \<tycolon> H1\<^sub>m)
+    \<Longrightarrow> \<^bold>c\<^bold>a\<^bold>s\<^bold>t h \<tycolon> H \<longmapsto> (x, h2) \<tycolon> \<medium_left_bracket> X <heap-sep> H2 \<medium_right_bracket> \<^bold>w\<^bold>i\<^bold>t\<^bold>h P1 \<and> P2 \<^bold>d\<^bold>u\<^bold>a\<^bold>l (x\<^sub>m, h2\<^sub>m) \<tycolon> \<medium_left_bracket> X\<^sub>m <heap-sep> H2\<^sub>m \<medium_right_bracket> \<longmapsto> h\<^sub>m \<tycolon> H\<^sub>m"
   unfolding Cast_def CastDual_def Heap_Cast_Goal_def SepNu_2_SepSet Intro_def Dest_def
   by (smt (verit, del_insts) SeparationSet_assoc SeparationSet_comm SeparationSet_def mem_Collect_eq)
 
-lemma [ \<nu>intro' ]: "\<^bold>d\<^bold>e\<^bold>s\<^bold>t \<^bold>c\<^bold>a\<^bold>s\<^bold>t x \<tycolon> T \<longmapsto> d \<tycolon> D \<^bold>w\<^bold>i\<^bold>t\<^bold>h P \<^bold>w\<^bold>h\<^bold>e\<^bold>n P' \<Longrightarrow> Different (x \<tycolon> T) (d \<tycolon> D) \<Longrightarrow> \<^bold>p\<^bold>r\<^bold>e\<^bold>m\<^bold>i\<^bold>s\<^bold>e P'
-  \<Longrightarrow> \<^bold>c\<^bold>a\<^bold>s\<^bold>t d \<tycolon> D \<longmapsto> d' \<tycolon> D' \<heavy_asterisk> h \<tycolon> \<medium_left_bracket> H \<medium_right_bracket> \<^bold>w\<^bold>i\<^bold>t\<^bold>h P2 \<^bold>d\<^bold>u\<^bold>a\<^bold>l i'\<^sub>m \<tycolon> I'\<^sub>m \<heavy_asterisk> h\<^sub>m \<tycolon> \<medium_left_bracket> H\<^sub>m \<medium_right_bracket> \<longmapsto> i \<tycolon> I \<^bold>w\<^bold>h\<^bold>e\<^bold>n Q2  
-  \<Longrightarrow> \<^bold>i\<^bold>n\<^bold>t\<^bold>r\<^bold>o \<^bold>c\<^bold>a\<^bold>s\<^bold>t i \<tycolon> I \<longmapsto> x\<^sub>m \<tycolon> T \<^bold>w\<^bold>i\<^bold>t\<^bold>h Q' \<^bold>w\<^bold>h\<^bold>e\<^bold>n Q
-  \<Longrightarrow> \<^bold>c\<^bold>a\<^bold>s\<^bold>t x \<tycolon> T \<longmapsto> d' \<tycolon> D' \<heavy_asterisk> h \<tycolon> \<medium_left_bracket> H \<medium_right_bracket> \<^bold>w\<^bold>i\<^bold>t\<^bold>h P \<and> P2 \<^bold>d\<^bold>u\<^bold>a\<^bold>l i'\<^sub>m \<tycolon> I'\<^sub>m \<heavy_asterisk> h\<^sub>m \<tycolon> \<medium_left_bracket> H\<^sub>m \<medium_right_bracket> \<longmapsto> x\<^sub>m \<tycolon> T \<^bold>w\<^bold>h\<^bold>e\<^bold>n Q \<and> Q2"
+lemma [ \<nu>intro' ]: "\<^bold>d\<^bold>e\<^bold>s\<^bold>t \<^bold>c\<^bold>a\<^bold>s\<^bold>t x \<tycolon> T \<longmapsto> d \<tycolon> D \<^bold>w\<^bold>i\<^bold>t\<^bold>h P
+  \<Longrightarrow> (P \<Longrightarrow> \<^bold>c\<^bold>a\<^bold>s\<^bold>t d \<tycolon> D \<longmapsto> d' \<tycolon> D' \<heavy_asterisk> h \<tycolon> \<medium_left_bracket> H \<medium_right_bracket> \<^bold>w\<^bold>i\<^bold>t\<^bold>h P2 \<^bold>d\<^bold>u\<^bold>a\<^bold>l i'\<^sub>m \<tycolon> I'\<^sub>m \<heavy_asterisk> h\<^sub>m \<tycolon> \<medium_left_bracket> H\<^sub>m \<medium_right_bracket> \<longmapsto> i \<tycolon> I)
+  \<Longrightarrow> (P \<Longrightarrow> P2 \<Longrightarrow> \<^bold>i\<^bold>n\<^bold>t\<^bold>r\<^bold>o \<^bold>c\<^bold>a\<^bold>s\<^bold>t i \<tycolon> I \<longmapsto> x\<^sub>m \<tycolon> T \<^bold>w\<^bold>i\<^bold>t\<^bold>h Anyway)
+  \<Longrightarrow> \<^bold>c\<^bold>a\<^bold>s\<^bold>t x \<tycolon> T \<longmapsto> d' \<tycolon> D' \<heavy_asterisk> h \<tycolon> \<medium_left_bracket> H \<medium_right_bracket> \<^bold>w\<^bold>i\<^bold>t\<^bold>h P \<and> P2 \<^bold>d\<^bold>u\<^bold>a\<^bold>l i'\<^sub>m \<tycolon> I'\<^sub>m \<heavy_asterisk> h\<^sub>m \<tycolon> \<medium_left_bracket> H\<^sub>m \<medium_right_bracket> \<longmapsto> x\<^sub>m \<tycolon> T"
   unfolding Dest_def Intro_def CastDual_def Different_def Heap_Cast_Goal_def Cast_def
   by (auto simp add: Premise_def)
 
@@ -637,7 +672,7 @@ subsection \<open>Cast\<close>
 
 theorem apply_cast: "(\<^bold>c\<^bold>u\<^bold>r\<^bold>r\<^bold>e\<^bold>n\<^bold>t blk \<^bold>r\<^bold>e\<^bold>s\<^bold>u\<^bold>l\<^bold>t\<^bold>s \<^bold>i\<^bold>n (R \<heavy_comma> x \<tycolon> X\<heavy_comma> \<^bold>h\<^bold>e\<^bold>a\<^bold>p H)) \<Longrightarrow> (\<^bold>c\<^bold>a\<^bold>s\<^bold>t x \<tycolon> X \<longmapsto> y \<tycolon> Y \<^bold>w\<^bold>i\<^bold>t\<^bold>h P) \<Longrightarrow> (\<^bold>c\<^bold>u\<^bold>r\<^bold>r\<^bold>e\<^bold>n\<^bold>t blk \<^bold>r\<^bold>e\<^bold>s\<^bold>u\<^bold>l\<^bold>t\<^bold>s \<^bold>i\<^bold>n (R \<heavy_comma> y \<tycolon> Y\<heavy_comma> \<^bold>h\<^bold>e\<^bold>a\<^bold>p H) \<and> P)"
   unfolding Procedure_def CurrentConstruction_def PendingConstruction_def bind_def SpecTop_imp Cast_def by (auto 4 6) 
-theorem "cast": "\<^bold>c\<^bold>u\<^bold>r\<^bold>r\<^bold>e\<^bold>n\<^bold>t blk \<^bold>r\<^bold>e\<^bold>s\<^bold>u\<^bold>l\<^bold>t\<^bold>s \<^bold>i\<^bold>n T \<Longrightarrow> \<^bold>c\<^bold>a\<^bold>s\<^bold>t T \<longmapsto> T' \<^bold>w\<^bold>i\<^bold>t\<^bold>h P \<^bold>w\<^bold>h\<^bold>e\<^bold>n Q \<Longrightarrow> \<^bold>p\<^bold>r\<^bold>e\<^bold>m\<^bold>i\<^bold>s\<^bold>e Q \<Longrightarrow> \<^bold>c\<^bold>u\<^bold>r\<^bold>r\<^bold>e\<^bold>n\<^bold>t blk \<^bold>r\<^bold>e\<^bold>s\<^bold>u\<^bold>l\<^bold>t\<^bold>s \<^bold>i\<^bold>n T' "
+theorem "cast": "\<^bold>c\<^bold>u\<^bold>r\<^bold>r\<^bold>e\<^bold>n\<^bold>t blk \<^bold>r\<^bold>e\<^bold>s\<^bold>u\<^bold>l\<^bold>t\<^bold>s \<^bold>i\<^bold>n T \<Longrightarrow> \<^bold>c\<^bold>a\<^bold>s\<^bold>t T \<longmapsto> T' \<^bold>w\<^bold>i\<^bold>t\<^bold>h P \<Longrightarrow> \<^bold>c\<^bold>u\<^bold>r\<^bold>r\<^bold>e\<^bold>n\<^bold>t blk \<^bold>r\<^bold>e\<^bold>s\<^bold>u\<^bold>l\<^bold>t\<^bold>s \<^bold>i\<^bold>n T' "
   for T' :: "(heap \<times> 'a::lrep) set" unfolding Cast_def CurrentConstruction_def by auto
 
 (* theorem proc_cast': "\<^bold>p\<^bold>r\<^bold>o\<^bold>c f \<blangle> A \<longmapsto> B \<brangle> \<Longrightarrow> \<^bold>c\<^bold>a\<^bold>s\<^bold>t A' \<longmapsto> A \<^bold>w\<^bold>i\<^bold>t\<^bold>h P \<Longrightarrow> \<^bold>c\<^bold>a\<^bold>s\<^bold>t B \<longmapsto> B' \<^bold>w\<^bold>i\<^bold>t\<^bold>h Q \<Longrightarrow> \<^bold>p\<^bold>r\<^bold>o\<^bold>c f \<blangle> A' \<longmapsto> B' \<brangle>"
@@ -659,9 +694,10 @@ lemma conversion: "\<^bold>c\<^bold>o\<^bold>n\<^bold>v\<^bold>e\<^bold>r\<^bold
 
 lemma [\<nu>intro0]: "\<^bold>c\<^bold>o\<^bold>n\<^bold>v\<^bold>e\<^bold>r\<^bold>s\<^bold>i\<^bold>o\<^bold>n f \<blangle> U \<longmapsto> V \<brangle> \<long_dobule_mapsto> f \<blangle> U \<longmapsto> V \<brangle>" unfolding Conversion_def by fast
 
-lemma conversion_cast[\<nu>intro]: "\<^bold>c\<^bold>a\<^bold>s\<^bold>t U' \<longmapsto> U \<^bold>w\<^bold>i\<^bold>t\<^bold>h P \<^bold>d\<^bold>u\<^bold>a\<^bold>l V \<longmapsto> V' \<^bold>w\<^bold>h\<^bold>e\<^bold>n Q \<Longrightarrow> \<^bold>p\<^bold>r\<^bold>e\<^bold>m\<^bold>i\<^bold>s\<^bold>e (P \<longrightarrow> Q) \<Longrightarrow> \<^bold>c\<^bold>o\<^bold>n\<^bold>v\<^bold>e\<^bold>r\<^bold>s\<^bold>i\<^bold>o\<^bold>n f \<blangle> U \<longmapsto> V \<brangle> \<long_dobule_mapsto> f \<blangle> U' \<longmapsto> V'\<brangle>"
-  unfolding Conversion_def Procedure_def Cast_def CastDual_def id_def Intro_def Dest_def
-  by (metis Cast_def CurrentConstruction_def LooseStateTy_introByStrict LooseStateTy_upgrade Premise_def "cast")
+lemma conversion_cast[\<nu>intro]: "\<^bold>c\<^bold>a\<^bold>s\<^bold>t U' \<longmapsto> U \<^bold>w\<^bold>i\<^bold>t\<^bold>h P \<^bold>d\<^bold>u\<^bold>a\<^bold>l V \<longmapsto> V' \<Longrightarrow> \<^bold>c\<^bold>o\<^bold>n\<^bold>v\<^bold>e\<^bold>r\<^bold>s\<^bold>i\<^bold>o\<^bold>n f \<blangle> U \<longmapsto> V \<brangle> \<long_dobule_mapsto> f \<blangle> U' \<longmapsto> V'\<brangle>"
+  unfolding Conversion_def Procedure_def Cast_def CastDual_def Intro_def Dest_def
+  by (metis LooseStateTy_introByStrict LooseStateTy_upgrade StrictStateTy_elim StrictStateTy_intro)
+
 (* lemma [\<nu>intro]: "\<^bold>p\<^bold>r\<^bold>o\<^bold>c g \<blangle> U' \<longmapsto> U \<brangle> \<Longrightarrow> \<^bold>c\<^bold>o\<^bold>n\<^bold>v\<^bold>e\<^bold>r\<^bold>s\<^bold>i\<^bold>o\<^bold>n f \<blangle> U \<longmapsto> V \<brangle> \<long_dobule_mapsto> (g \<nuInstrComp> f) \<blangle> U' \<longmapsto> V\<brangle>"
   unfolding Conversion_def using instr_comp by fast *)
 
@@ -879,9 +915,8 @@ ML_file "./library/processor.ML"
 ML_file "./library/procedure.ML"
 ML_file "./library/exty.ML"
 ML_file NuSys.ML
-(* ML_file "./library/registers.ML" *)
 ML_file "./library/processors.ML"
-(* ML_file "./library/obtain.ML" *)
+ML_file "./library/obtain.ML"
 ML_file NuToplevel.ML 
 
 section \<open>Attributes and Commands\<close>
@@ -1044,7 +1079,7 @@ attribute_setup \<nu>cast_overload = \<open>Scan.lift (Parse.and_list1 NuProcedu
 
 section \<open>Processors\<close>
 
-subsubsection \<open>Controls\<close>
+subsection \<open>Controls\<close>
 
 \<nu>processor set_auto_level 10 \<open>PROP P\<close> \<open>(fn ctx => fn th => NuParse.auto_level_force #->
   (fn auto_level' => NuProcessor.process (AutoLevel.reduce auto_level' ctx) th #> (fn x => raise ProcessTerminated x)))\<close>
@@ -1056,7 +1091,7 @@ subsubsection \<open>Controls\<close>
         (NuProcessor.process ctx #> (fn p => p [tok,Token.eof] |> #1)) th)
   end\<close>
 
-subsubsection \<open>Essential functions\<close>
+subsection \<open>Essential functions\<close>
 
 \<nu>processor accept_proc 300 \<open>\<^bold>p\<^bold>e\<^bold>n\<^bold>d\<^bold>i\<^bold>n\<^bold>g f \<^bold>o\<^bold>n blk \<^bold>r\<^bold>e\<^bold>s\<^bold>u\<^bold>l\<^bold>t\<^bold>s \<^bold>i\<^bold>n T\<close> \<open>fn ctx => fn th => Scan.succeed (fn _ => NuSys.accept_proc ctx th)\<close>
 
@@ -1092,7 +1127,7 @@ val ctx = NuSys.load_specthm meta ctx
     case Thm.biresolution NONE false (ths |> map (pair false) |> @{print}) 1 major |> Seq.pull
       of SOME (th, _) => th | _ => raise THM ("RSN: no unifiers", 1, major::ths)) |> intro_SPEC end)\<close>
 
-\<nu>processor rule_by_COMP 1000 \<open>PROP P \<Longrightarrow> PROP Q\<close>
+(* \<nu>processor rule_by_COMP 1000 \<open>PROP P \<Longrightarrow> PROP Q\<close>
   \<open>fn ctx => fn meta => (Parse.$$$ "\<Longleftarrow>'" |-- NuProcedure.parser -- Parse.opt_attribs) >> (fn (name,attrs) => fn _ =>
     let open NuBasics
     val ctx = NuSys.load_specthm meta ctx
@@ -1100,15 +1135,18 @@ val ctx = NuSys.load_specthm meta ctx
     val [th] = Proof_Context.get_fact ctx (Facts.Named (name, NONE)) 
     val ([th],ctx) = fold_map (Thm.proof_attributes attrs) [th] ctx
     in elim_SPEC meta |> apfst (fn major => th COMP major) |> intro_SPEC end)\<close>
+*)
 
 \<nu>processor set_\<nu>current 100 \<open>\<^bold>c\<^bold>u\<^bold>r\<^bold>r\<^bold>e\<^bold>n\<^bold>t blk \<^bold>r\<^bold>e\<^bold>s\<^bold>u\<^bold>l\<^bold>t\<^bold>s \<^bold>i\<^bold>n T\<close> \<open>fn ctx => fn meta => Scan.succeed (fn _ =>
   raise Bypass (SOME (meta RS @{thm set_\<nu>current})))\<close>
 
-(* \<nu>processor choose_AutoExTy 10 \<open>\<^bold>c\<^bold>u\<^bold>r\<^bold>r\<^bold>e\<^bold>n\<^bold>t blk \<^bold>r\<^bold>e\<^bold>s\<^bold>u\<^bold>l\<^bold>t\<^bold>s \<^bold>i\<^bold>n AutoExTyp T\<close> \<open>fn ctx => fn meta =>
-  Parse.list1 Parse.binding >> (fn vars => fn () =>
-    raise Process_State_Call' (meta, NuObtain.chooseV vars))\<close> *)
+subsubsection \<open>Existential elimination\<close>
 
-subsubsection \<open>Simplifiers & Resonings\<close>
+\<nu>processor auto_existential_elimination 50 \<open>\<^bold>c\<^bold>u\<^bold>r\<^bold>r\<^bold>e\<^bold>n\<^bold>t blk \<^bold>r\<^bold>e\<^bold>s\<^bold>u\<^bold>l\<^bold>t\<^bold>s \<^bold>i\<^bold>n \<tort_lbrace>x \<tycolon> ExNu T\<tort_rbrace>\<close>
+  \<open>fn ctx => fn meta => Scan.succeed (fn () =>
+    raise Process_State_Call' (meta, NuObtain.auto_choose))\<close>
+
+subsection \<open>Simplifiers & Resonings\<close>
 
 \<nu>processor \<nu>simplifier 40 \<open>\<^bold>c\<^bold>u\<^bold>r\<^bold>r\<^bold>e\<^bold>n\<^bold>t blk \<^bold>r\<^bold>e\<^bold>s\<^bold>u\<^bold>l\<^bold>t\<^bold>s \<^bold>i\<^bold>n T\<close>  \<open>NuProcessors.simplifier []\<close>
 (* \<nu>processor \<nu>simplifier_final 9999 \<open>PROP P\<close>  \<open>NuProcessors.simplifier []\<close> *)
@@ -1117,7 +1155,7 @@ subsubsection \<open>Simplifiers & Resonings\<close>
   NuSys.auto_resolve_rule NONE [] (NuSys.load_specthm meta ctx) meta
     handle NuSys.ReasoningFail _ => raise Bypass NONE)\<close>
 
-subsubsection \<open>Literal operations\<close>
+subsection \<open>Literal operations\<close>
 
 \<nu>processor literal_constructor 9500 \<open>\<^bold>c\<^bold>u\<^bold>r\<^bold>r\<^bold>e\<^bold>n\<^bold>t blk \<^bold>r\<^bold>e\<^bold>s\<^bold>u\<^bold>l\<^bold>t\<^bold>s \<^bold>i\<^bold>n T\<close> \<open>fn ctx => fn meta => Parse.cartouche >> (fn term => fn _ =>
   let val term = Syntax.read_term ctx term |> Thm.cterm_of ctx |> Simplifier.rewrite ctx |> Thm.rhs_of
