NuBasicAbstractors.thy
@@ -39,7 +39,7 @@ notation NuRefine (infixl "<where>" 80)
 lemma [simp]: " p \<nuLinkL> N \<nuRefine> P \<nuLinkR> x \<longleftrightarrow> x \<in> P \<and> ( p \<nuLinkL> N \<nuLinkR> x)" unfolding NuRefine_def Refining_def by auto
 lemma [elim,\<nu>elim]: " x \<ratio> N \<nuRefine> P \<Longrightarrow> (x \<in> P \<Longrightarrow> x \<ratio> N \<Longrightarrow> C) \<Longrightarrow> C" unfolding Inhabited_def by auto
 
-lemma [\<nu>intro]: "\<^bold>i\<^bold>n\<^bold>t\<^bold>r\<^bold>o \<^bold>c\<^bold>a\<^bold>s\<^bold>t x \<tycolon> M \<longmapsto> x \<tycolon> M <where> S \<^bold>w\<^bold>h\<^bold>e\<^bold>n x \<in> S"
+lemma [\<nu>intro]: "\<^bold>p\<^bold>r\<^bold>e\<^bold>m\<^bold>i\<^bold>s\<^bold>e x \<in> S \<Longrightarrow> \<^bold>i\<^bold>n\<^bold>t\<^bold>r\<^bold>o \<^bold>c\<^bold>a\<^bold>s\<^bold>t x \<tycolon> M \<longmapsto> x \<tycolon> M <where> S"
   unfolding Intro_def Cast_def by auto
 lemma [\<nu>intro]: "\<^bold>d\<^bold>e\<^bold>s\<^bold>t \<^bold>c\<^bold>a\<^bold>s\<^bold>t x \<tycolon> M <where> S \<longmapsto> x \<tycolon> M \<^bold>w\<^bold>i\<^bold>t\<^bold>h x \<in> S"
   unfolding Dest_def Cast_def by auto
@@ -76,7 +76,7 @@ lemma [elim,\<nu>elim]: " x \<ratio> N <down-lift> g \<Longrightarrow> ( g x \<r
 (* lemma [\<nu>cast_overload E]: " \<^bold>c\<^bold>a\<^bold>s\<^bold>t x \<tycolon> N <down-lift> g \<longmapsto> g x \<tycolon> N" unfolding Cast_def by simp *)
 lemma [\<nu>intro]: "\<^bold>p\<^bold>r\<^bold>e\<^bold>m\<^bold>i\<^bold>s\<^bold>e g x = x' \<Longrightarrow> \<^bold>c\<^bold>a\<^bold>s\<^bold>t x \<tycolon> N <down-lift> g \<longmapsto> x' \<tycolon> N" unfolding Cast_def by auto
 
-lemma [\<nu>intro]: "\<^bold>i\<^bold>n\<^bold>t\<^bold>r\<^bold>o \<^bold>c\<^bold>a\<^bold>s\<^bold>t x \<tycolon> M \<longmapsto> y \<tycolon> M <down-lift> g \<^bold>w\<^bold>h\<^bold>e\<^bold>n (g y = x)"
+lemma [\<nu>intro]: "\<^bold>p\<^bold>r\<^bold>e\<^bold>m\<^bold>i\<^bold>s\<^bold>e (g y = x) \<Longrightarrow> \<^bold>i\<^bold>n\<^bold>t\<^bold>r\<^bold>o \<^bold>c\<^bold>a\<^bold>s\<^bold>t x \<tycolon> M \<longmapsto> y \<tycolon> M <down-lift> g"
   unfolding Intro_def Cast_def by auto
 lemma [\<nu>intro]: "\<^bold>d\<^bold>e\<^bold>s\<^bold>t \<^bold>c\<^bold>a\<^bold>s\<^bold>t y \<tycolon> M <down-lift> g \<longmapsto> g y \<tycolon> M"
   unfolding Dest_def Cast_def by auto
@@ -111,7 +111,7 @@ lemma [elim,\<nu>elim]: " x \<ratio> N <up-lift> f \<Longrightarrow> (\<And>y. f
 
 lemma [\<nu>intro]: "\<^bold>i\<^bold>n\<^bold>t\<^bold>r\<^bold>o \<^bold>c\<^bold>a\<^bold>s\<^bold>t x \<tycolon> M \<longmapsto> g x \<tycolon> M <up-lift> g"
   unfolding Intro_def Cast_def by auto
-lemma [\<nu>intro]: "(\<And> x.  (g x = y) \<Longrightarrow> \<^bold>d\<^bold>e\<^bold>s\<^bold>t \<^bold>c\<^bold>a\<^bold>s\<^bold>t x \<tycolon> M \<longmapsto> N \<^bold>w\<^bold>i\<^bold>t\<^bold>h P \<^bold>w\<^bold>h\<^bold>e\<^bold>n Q) \<Longrightarrow> \<^bold>d\<^bold>e\<^bold>s\<^bold>t \<^bold>c\<^bold>a\<^bold>s\<^bold>t y \<tycolon> M <up-lift> g \<longmapsto> N \<^bold>w\<^bold>i\<^bold>t\<^bold>h P \<^bold>w\<^bold>h\<^bold>e\<^bold>n Q"
+lemma [\<nu>intro]: "(\<And> x.  (g x = y) \<Longrightarrow> \<^bold>d\<^bold>e\<^bold>s\<^bold>t \<^bold>c\<^bold>a\<^bold>s\<^bold>t x \<tycolon> M \<longmapsto> N \<^bold>w\<^bold>i\<^bold>t\<^bold>h P) \<Longrightarrow> \<^bold>d\<^bold>e\<^bold>s\<^bold>t \<^bold>c\<^bold>a\<^bold>s\<^bold>t y \<tycolon> M <up-lift> g \<longmapsto> N \<^bold>w\<^bold>i\<^bold>t\<^bold>h P"
   unfolding Dest_def Cast_def by auto
 
 lemma "\<^bold>d\<^bold>e\<^bold>s\<^bold>t \<^bold>c\<^bold>a\<^bold>s\<^bold>t y \<tycolon> M <up-lift> g \<longmapsto> (\<exists>* x. x \<tycolon> M \<and>\<^sup>\<nu> (g x = y))"
@@ -244,12 +244,8 @@ lemma [simp]: "i < length l \<Longrightarrow> mapSome l ! i = Some (l ! i)" unfo
 lemma [simp]: "i < length l \<Longrightarrow> (mapSome l) [i := Some v] = mapSome (l [i:=v])" unfolding mapSome_def by (metis map_update)
 lemma [simp]: "i < length l \<Longrightarrow> the (mapSome l ! i) = l ! i" unfolding mapSome_def by auto
 
-lemma cast_dual_trans: 
-  "\<^bold>c\<^bold>a\<^bold>s\<^bold>t A \<longmapsto> B \<^bold>w\<^bold>i\<^bold>t\<^bold>h P1 \<^bold>d\<^bold>u\<^bold>a\<^bold>l B' \<longmapsto> A' \<^bold>w\<^bold>h\<^bold>e\<^bold>n Q1 \<Longrightarrow> \<^bold>c\<^bold>a\<^bold>s\<^bold>t B \<longmapsto> C \<^bold>w\<^bold>i\<^bold>t\<^bold>h P2 \<^bold>d\<^bold>u\<^bold>a\<^bold>l C' \<longmapsto> B' \<^bold>w\<^bold>h\<^bold>e\<^bold>n Q2
-    \<Longrightarrow> \<^bold>c\<^bold>a\<^bold>s\<^bold>t A \<longmapsto> C \<^bold>w\<^bold>i\<^bold>t\<^bold>h P1 \<and> P2 \<^bold>d\<^bold>u\<^bold>a\<^bold>l C' \<longmapsto> A' \<^bold>w\<^bold>h\<^bold>e\<^bold>n Q1 \<and> Q2"
-  unfolding Cast_def CastDual_def Intro_def Dest_def by auto
 
-lemma [\<nu>intro]: "\<^bold>i\<^bold>n\<^bold>t\<^bold>r\<^bold>o \<^bold>c\<^bold>a\<^bold>s\<^bold>t  a \<R_arr_tail> xs' \<tycolon> Array' N \<longmapsto> a \<R_arr_tail> xs2 \<tycolon> Array N \<^bold>w\<^bold>h\<^bold>e\<^bold>n xs' = mapSome xs2"
+lemma [\<nu>intro]: "\<^bold>p\<^bold>r\<^bold>e\<^bold>m\<^bold>i\<^bold>s\<^bold>e xs' = mapSome xs2 \<Longrightarrow> \<^bold>i\<^bold>n\<^bold>t\<^bold>r\<^bold>o \<^bold>c\<^bold>a\<^bold>s\<^bold>t  a \<R_arr_tail> xs' \<tycolon> Array' N \<longmapsto> a \<R_arr_tail> xs2 \<tycolon> Array N"
   unfolding Cast_def Intro_def Array_def by (cases a) (auto simp add: pred_option_def Ball_def)
 lemma [\<nu>intro]: "\<^bold>d\<^bold>e\<^bold>s\<^bold>t \<^bold>c\<^bold>a\<^bold>s\<^bold>t a \<R_arr_tail> xs \<tycolon> Array N \<longmapsto> a \<R_arr_tail> mapSome xs \<tycolon> Array' N"
   unfolding Cast_def Dest_def Array_def by (cases a) (auto simp add: pred_option_def Ball_def)
